

# Homotopy Type Theory

## Basics

### 2.1 Types are higher groupoids

**Lemma 2.1.1.** For every type  $A$  and every  $x, y : A$  there is a function

$$(x = y) \rightarrow (y = x)$$

denoted  $p \mapsto p^{-1}$ , such that  $\text{refl}_x^{-1} \equiv \text{refl}_x$  for each  $x : A$ . We call  $p^{-1}$  the *inverse* of  $p$ .

**Lemma 2.1.2.** For every type  $A$  and every  $x, y, z : A$  there is a function

$$(x = y) \rightarrow (y = z) \rightarrow (x = z)$$

written  $p \mapsto q \mapsto p \cdot q$ , such that  $\text{refl}_x \cdot \text{refl}_x \equiv \text{refl}_x$  for any  $x : A$ . We call  $p \cdot q$  the *concatenation* or *composite* of  $p$  and  $q$ .

Equality	Homotopy	$\infty$ -Groupoid
reflexivity	constant path	identity morphism
symmetry	inversion of paths	inverse morphism
transitivity	concatenation of paths	composition of morphisms

**Lemma 2.1.3.** Suppose  $A : \mathcal{U}$ , that  $x, y, z, w : A$  and that  $p : x = y$  and  $q : y = z$  and  $r : z = w$ . We have the following:

- (i)  $p = p \cdot \text{refl}_y$  and  $p = \text{refl}_x \cdot p$ .
- (ii)  $p^{-1} \cdot p = \text{refl}_y$  and  $p \cdot p^{-1} = \text{refl}_x$ .
- (iii)  $(p^{-1})^{-1} = p$ .
- (iv)  $p \cdot (q \cdot r) = (p \cdot q) \cdot r$ .

**Theorem 2.1.4** (Eckmann–Hilton). The composition operation on the second loop space

$$\Omega^2(A) \times \Omega^2(A) \rightarrow \Omega^2(A)$$

is commutative:  $\alpha \cdot \beta = \beta \cdot \alpha$ , for any  $\alpha, \beta : \Omega^2(A)$ .

**Definition 2.1.5.** A **pointed type**  $(A, a)$  is a type  $A : \mathcal{U}$  together with a point  $a : A$ , called its **basepoint**. We write  $\mathbf{U}_\bullet := \sum_{(A, a)} A$  for the type of pointed types in the universe  $\mathcal{U}$ .

**Definition 2.1.6.** Given a pointed type  $(A, a)$ , we define the **loop space** of  $(A, a)$  to be the following pointed type:

$$\Omega(A, a) := ((a =_A a), \text{refl}_a).$$

An element of it will be called a **loop** at  $a$ . For  $n : \mathbb{N}$ , the  **$n$ -fold iterated loop space**  $\Omega^n(A, a)$  of a pointed type  $(A, a)$  is defined recursively by:

$$\Omega^0(A, a) := (A, a)$$

$$\Omega^{n+1}(A, a) := \Omega^n(\Omega(A, a)).$$

An element of it will be called an  **$n$ -loop** or an  **$n$ -dimensional loop** at  $a$ .

### 2.2 Functions are functors

**Lemma 2.2.1.** Suppose that  $f : A \rightarrow B$  is a function. Then for any  $x, y : A$  there is an operation

$$\text{ap}_f : (x =_A y) \rightarrow (f(x) =_B f(y)).$$

Moreover, for each  $x : A$  we have  $\text{ap}_f(\text{refl}_x) \equiv \text{refl}_{f(x)}$ .

The notation  $\text{ap}_f$  can be read either as the application of  $f$  to a path, or as the action on paths of  $f$ .

We note that  $\text{ap}$  behaves functorially, in all the ways that one might expect.

**Lemma 2.2.2.** For functions  $f : A \rightarrow B$  and  $g : B \rightarrow C$  and paths  $p : x =_A y$  and  $q : y =_B z$ , we have:

- (i)  $\text{ap}_f(p \cdot q) = \text{ap}_f(p) \cdot \text{ap}_f(q)$ .
- (ii)  $\text{ap}_f(p^{-1}) = \text{ap}_f(p)^{-1}$ .
- (iii)  $\text{ap}_g(\text{ap}_f(p)) = \text{ap}_{g \circ f}(p)$ .
- (iv)  $\text{ap}_{\text{id}_A}(p) = p$ .

### 2.3 Type families are fibrations

**Lemma 2.3.1** (Transport). Suppose that  $P$  is a type family over  $A$  and that  $p : x =_A y$ . Then there is a function  $p_* : P(x) \rightarrow P(y)$ .

Sometimes, it is necessary to notate the type family  $P$  in which the transport operation happens.

$$\text{transport}^P(p, -) : P(x) \rightarrow P(y).$$

**Lemma 2.3.2** (Path lifting property). Let  $P : A \rightarrow \mathcal{U}$  be a type family over  $A$  and assume we have  $u : P(x)$  for some  $x : A$ . Then for any  $p : x = y$ , we have

$$\text{lift}(u, p) : (x, u) = (y, p_*(u))$$

in  $\sum_{(x:A)} P(x)$ , such that  $\text{pr}_1(\text{lift}(u, p)) = p$ .

**Remark 2.3.3.** Although we may think of a type family  $P : A \rightarrow \mathcal{U}$  as like a fibration, it is generally not a good idea to say things like “the fibration  $P : A \rightarrow \mathcal{U}$ ”, since this sounds like we are talking about a fibration with base  $\mathcal{U}$  and total space  $A$ . To repeat, when a type family  $P : A \rightarrow \mathcal{U}$  is regarded as a fibration, the base is  $A$  and the total space is  $\sum_{(x:A)} P(x)$ . We may also occasionally use other topological terminology when speaking about type families. For instance, we may refer to a dependent function  $f : \prod_{(x:A)} P(x)$  as a **section** of the fibration  $P$ , and we may say that something happens **fiberwise** if it happens for each  $P(x)$ . For instance, a section  $f : \prod_{(x:A)} P(x)$  shows that  $P$  is “fiberwise inhabited”.

**Lemma 2.3.4** (Dependent map). Suppose  $f : \prod_{(x:A)} P(x)$ ; then we have a map

$$\text{apd}_f : \prod_{p:x=y} (p_*(f(x)) =_{P(y)} f(y)).$$

**Lemma 2.3.5.** If  $P : A \rightarrow \mathcal{U}$  is defined by  $P(x) := B$  for a fixed  $B : \mathcal{U}$ , then for any  $x, y : A$  and  $p : x = y$  and  $b : B$  we have a path

$$\text{transportconst}_p^B(b) : \text{transport}^P(p, b) = b.$$

**Lemma 2.3.6.** For  $f : A \rightarrow B$  and  $p : x =_A y$ , we have

$$\text{apd}_f(p) = \text{transportconst}_p^B(f(x)) \cdot \text{ap}_f(p).$$

**Lemma 2.3.7.** Given  $P : A \rightarrow \mathcal{U}$  with  $p : x =_A y$  and  $q : y =_A z$  while  $u : P(x)$ , we have

$$q_*(p_*(u)) = (p \cdot q)_*(u).$$

**Lemma 2.3.8.** For a function  $f : A \rightarrow B$  and a type family  $P : B \rightarrow \mathcal{U}$ , and any  $p : x =_A y$  and  $u : P(f(x))$ , we have

$$\text{transport}^{P \circ f}(p, u) = \text{transport}^P(\text{ap}_f(p), u).$$

**Lemma 2.3.9.** For  $P, Q : A \rightarrow \mathcal{U}$  and a family of functions  $f : \prod_{(x:A)} P(x) \rightarrow Q(x)$ , and any  $p : x =_A y$  and  $u : P(x)$ , we have

$$\text{transport}^Q(p, f_x(u)) = f_y(\text{transport}^P(p, u)).$$

### 2.4 Homotopies and equivalences

**Definition 2.4.1.** Let  $f, g : \prod_{(x:A)} P(x)$  be two sections of a type family  $P : A \rightarrow \mathcal{U}$ . A **homotopy** from  $f$  to  $g$  is a dependent function of type

$$(f \sim g) := \prod_{x:A} (f(x) = g(x)).$$

Note that a homotopy is not the same as an identification ( $f = g$ ). However, in §2.9 we will introduce an axiom making homotopies and identifications “equivalent”.

The following proofs are left to the reader.

**Lemma 2.4.2.** Homotopy is an equivalence relation on each dependent function type  $\prod_{(x:A)} P(x)$ . That is, we have elements of the types

$$\begin{aligned} & \prod_{f:\prod_{(x:A)} P(x)} (f \sim f) \\ & \prod_{f,g:\prod_{(x:A)} P(x)} (f \sim g) \rightarrow (g \sim f) \\ & \prod_{f,g,h:\prod_{(x:A)} P(x)} (f \sim g) \rightarrow (g \sim h) \rightarrow (f \sim h). \end{aligned}$$

**Lemma 2.4.3.** Suppose  $H : f \sim g$  is a homotopy between functions  $f, g : A \rightarrow B$  and let  $p : x =_A y$ . Then we have

$$H(x) \cdot g(p) = f(p) \cdot H(y).$$

We may also draw this as a commutative diagram:

$$\begin{array}{ccc} f(x) & \xrightarrow{f(p)} & f(y) \\ \parallel^{H(x)} & & \parallel^{H(y)} \\ g(x) & \xrightarrow[g(p)]{} & g(y) \end{array}$$

**Corollary 2.4.4.** Let  $H : f \sim \text{id}_A$  be a homotopy, with  $f : A \rightarrow A$ . Then for any  $x : A$  we have

$$H(f(x)) = f(H(x)).$$

$$\sum_{g:B \rightarrow A} ((f \circ g \sim \text{id}_B) \times (g \circ f \sim \text{id}_A)) \quad (2.4.5)$$

**Definition 2.4.6.** For a function  $f : A \rightarrow B$ , a **quasi-inverse** of  $f$  is a triple  $(g, \alpha, \beta)$  consisting of a function  $g : B \rightarrow A$  and homotopies  $\alpha : f \circ g \sim \text{id}_B$  and  $\beta : g \circ f \sim \text{id}_A$ .

Thus, (2.4.5) is the type of quasi-inverses of  $f$ ; we may denote it by  $\text{qinv}(f)$ .

**Example 2.4.7.** For any  $p : x =_A y$  and  $z : A$ , the functions

$$(p \bullet -) : (y =_A z) \rightarrow (x =_A z) \quad \text{and} \\ (- \bullet p) : (z =_A x) \rightarrow (z =_A y)$$

have quasi-inverses given by  $(p^{-1} \bullet -)$  and  $(- \bullet p^{-1})$ , respectively;

**Example 2.4.8.** For any  $p : x =_A y$  and  $P : A \rightarrow \mathcal{U}$ , the function

$$\text{transport}^P(p, -) : P(x) \rightarrow P(y)$$

has a quasi-inverse given by  $\text{transport}^P(p^{-1}, -)$ ; this follows from Lemma 2.3.7.

$$(A \simeq B) := \sum_{f:A \rightarrow B} \text{isequiv}(f). \quad (2.4.9)$$

**Lemma 2.4.10.** Type equivalence is an equivalence relation on  $\mathcal{U}$ . More specifically:

- (i) For any  $A$ , the identity function  $\text{id}_A$  is an equivalence; hence  $A \simeq A$ .
- (ii) For any  $f : A \simeq B$ , we have an equivalence  $f^{-1} : B \simeq A$ .
- (iii) For any  $f : A \simeq B$  and  $g : B \simeq C$ , we have  $g \circ f : A \simeq C$ .

## 2.5 The higher groupoid structure of type formers

## 2.6 Cartesian product types

$$(x =_{A \times B} y) \rightarrow (\text{pr}_1(x) =_A \text{pr}_1(y)) \times (\text{pr}_2(x) =_B \text{pr}_2(y)). \quad (2.6.1)$$

**Theorem 2.6.2.** For any  $x$  and  $y$ , the function (2.6.1) is an equivalence.

**Theorem 2.6.3.** In the above situation, we have

$$\text{transport}^{A \times B}(p, x) =_{A(w) \times B(w)} (\text{transport}^A(p, \text{pr}_1 x), \text{transport}^B(p, \text{pr}_2 x)).$$

**Theorem 2.6.4.** In the above situation, given  $x, y : A \times B$  and  $p : \text{pr}_1 x = \text{pr}_1 y$  and  $q : \text{pr}_2 x = \text{pr}_2 y$ , we have

$$f(\text{pair}^=(p, q)) =_{(f(x)=f(y))} \text{pair}^=(g(p), h(q)).$$

## 2.7 $\Sigma$ -types

**Theorem 2.7.1.** Suppose that  $P : A \rightarrow \mathcal{U}$  is a type family over a type  $A$  and let  $w, w' : \sum_{(x:A)} P(x)$ . Then there is an equivalence

$$(w = w') \simeq \sum_{(p:\text{pr}_1(w)=\text{pr}_1(w'))} p_*(\text{pr}_2(w)) = \text{pr}_2(w').$$

**Corollary 2.7.2.** For  $z : \sum_{(x:A)} P(x)$ , we have  $z = (\text{pr}_1(z), \text{pr}_2(z))$ .

**Theorem 2.7.3.** Suppose we have type families

$$P : A \rightarrow \mathcal{U} \quad \text{and} \quad Q : \left( \sum_{x:A} P(x) \right) \rightarrow \mathcal{U}.$$

Then we can construct the type family over  $A$  defined by

$$x \mapsto \sum_{u:P(x)} Q(x, u).$$

For any path  $p : x = y$  and any  $(u, z) : \sum_{(u:P(x))} Q(x, u)$  we have

$$p_*(u, z) = (p_*(u), \text{pair}^=(p, \text{refl}_{p_*(u)})_*(z)).$$

## 2.8 The unit type

**Theorem 2.8.1.** For any  $x, y : \mathbf{1}$ , we have  $(x = y) \simeq \mathbf{1}$ .

## 2.9 $\Pi$ -types and the function extensionality axiom

$$\text{happly} : (f = g) \rightarrow \prod_{x:A} (f(x) =_{B(x)} g(x)) \quad (2.9.1)$$

**Axiom 2.9.2** (Function extensionality). For any  $A, B, f$ , and  $g$ , the function (2.9.1) is an equivalence.

In particular, Axiom 2.9.2 implies that (2.9.1) has a quasi-inverse

$$\text{funext} : \left( \prod_{x:A} (f(x) = g(x)) \right) \rightarrow (f = g).$$

This function is also referred to as “function extensionality”.

$$\text{refl}_f = \text{funext}(x \mapsto \text{refl}_{f(x)})$$

$$\alpha^{-1} = \text{funext}(x \mapsto \text{happly}(\alpha, x)^{-1})$$

$$\alpha \bullet \beta = \text{funext}(x \mapsto \text{happly}(\alpha, x) \bullet \text{happly}(\beta, x)).$$

Given a type  $X$ , a path  $p : x_1 =_X x_2$ , type families  $A, B : X \rightarrow \mathcal{U}$ , and a function  $f : A(x_1) \rightarrow B(x_1)$ , we have

$$\text{transport}^{A \rightarrow B}(p, f) = \left( x \mapsto \text{transport}^B(p, f(\text{transport}^A(p^{-1}, x))) \right) \quad (2.9.3)$$

where  $A \rightarrow B$  denotes abusively the type family  $X \rightarrow \mathcal{U}$  defined by

$$(A \rightarrow B)(x) \equiv (A(x) \rightarrow B(x)).$$

Transporting dependent functions is similar, but more complicated. Suppose given  $X$  and  $p$  as before, type families  $A : X \rightarrow \mathcal{U}$  and  $B : \prod_{(x:X)} (A(x) \rightarrow \mathcal{U})$ , and also a dependent function  $f : \prod_{(a:A(x_1))} B(x_1, a)$ . Then for  $a : A(x_2)$ , we have

$$\text{transport}^{\Pi_A(B)}(p, f)(a) = \text{transport}^{\hat{B}}\left(\left(\text{pair}^=(p^{-1}, \text{refl}_{p^{-1}_*(a)})\right)^{-1}, f(\text{transport}^A(p^{-1}, a))\right)$$

where  $\Pi_A(B)$  and  $\hat{B}$  denote respectively the type families

$$\begin{aligned} \Pi_A(B) &::= (x \mapsto \prod_{(a:A(x))} B(x, a)) & : X \rightarrow \mathcal{U} \\ \hat{B} &::= (w \mapsto B(\text{pr}_1 w, \text{pr}_2 w)) & : \left( \sum_{(x:X)} A(x) \right) \rightarrow \mathcal{U}. \end{aligned} \quad (2.9.4)$$

**Lemma 2.9.5.** Given type families  $A, B : X \rightarrow \mathcal{U}$  and  $p : x =_X y$ , and also  $f : A(x) \rightarrow B(x)$  and  $g : A(y) \rightarrow B(y)$ , we have an equivalence

$$(p_*(f) = g) \simeq \prod_{a:A(x)} (p_*(f(a)) = g(p_*(a))).$$

Moreover, if  $q : p_*(f) = g$  corresponds under this equivalence to  $\hat{q}$ , then for  $a : A(x)$ , the path

$$\text{happly}(q, p_*(a)) : (p_*(f))(p_*(a)) = g(p_*(a))$$

is equal to the concatenated path  $i \bullet j \bullet k$ , where

- $i : (p_*(f))(p_*(a)) = p_*(f(p^{-1}_*(p_*(a))))$  comes from (2.9.3),
- $j : p_*(f(p^{-1}_*(p_*(a)))) = p_*(f(a))$  comes from Lemmas 2.1.3 and 2.3.7, and
- $k : p_*(f(a)) = g(p_*(a))$  is  $\hat{q}(a)$ .

**Lemma 2.9.6.** Given type families  $A : X \rightarrow \mathcal{U}$  and  $B : \prod_{(x:X)} A(x) \rightarrow \mathcal{U}$  and  $p : x =_X y$ , and also  $f : \prod_{(a:A(x))} B(x, a)$  and  $g : \prod_{(a:A(y))} B(y, a)$ , we have an equivalence

$$(p_*(f) = g) \simeq \left( \prod_{a:A(x)} \text{transport}^{\hat{B}}(\text{pair}^=(p, \text{refl}_{p_*(a)}), f(a)) = g(p_*(a)) \right)$$

with  $\hat{B}$  as in (2.9.4).

## 2.10 Universes and the univalence axiom

**Lemma 2.10.1.** For types  $A, B : \mathcal{U}$ , there is a certain function,

$$\text{idtoeqv} : (A =_{\mathcal{U}} B) \rightarrow (A \simeq B), \quad (2.10.2)$$

defined in the proof.

**Axiom 2.10.3** (Univalence). For any  $A, B : \mathcal{U}$ , the function (2.10.2) is an equivalence.

- An introduction rule for  $(A =_{\mathcal{U}} B)$ , denoted  $\text{ua}$  for “univalence axiom”:

$$\text{ua} : (A \simeq B) \rightarrow (A =_{\mathcal{U}} B).$$

- The elimination rule, which is  $\text{idtoeqv}$ ,

$$\text{idtoeqv} \equiv \text{transport}^{X \mapsto X} : (A =_{\mathcal{U}} B) \rightarrow (A \simeq B).$$

- The propositional computation rule,

$$\text{transport}^{X \mapsto X}(\text{ua}(f), x) = f(x).$$

- The propositional uniqueness principle: for any  $p : A = B$ ,

$$p = \text{ua}(\text{transport}^{X \mapsto X}(p)).$$

We can also identify the reflexivity, concatenation, and inverses of equalities in the universe with the corresponding operations on equivalences:

$$\begin{aligned} \text{refl}_A &= \text{ua}(\text{id}_A) \\ \text{ua}(f) \cdot \text{ua}(g) &= \text{ua}(g \circ f) \\ \text{ua}(f)^{-1} &= \text{ua}(f^{-1}). \end{aligned}$$

**Lemma 2.10.4.** For any type family  $B : A \rightarrow \mathcal{U}$  and  $x, y : A$  with a path  $p : x = y$  and  $u : B(x)$ , we have

$$\begin{aligned} \text{transport}^B(p, u) &= \text{transport}^{X \mapsto X}(\text{ap}_B(p), u) \\ &= \text{idtoeqv}(\text{ap}_B(p))(u). \end{aligned}$$

## 2.11 Identity type

**Theorem 2.11.1.** If  $f : A \rightarrow B$  is an equivalence, then for all  $a, a' : A$ , so is

$$\text{ap}_f : (a =_A a') \rightarrow (f(a) =_B f(a')).$$

**Lemma 2.11.2.** For any  $A$  and  $a : A$ , with  $p : x_1 = x_2$ , we have

$$\begin{aligned} \text{transport}^{x \mapsto (a=x)}(p, q) &= q \cdot p && \text{for } q : a = x_1, \\ \text{transport}^{x \mapsto (x=a)}(p, q) &= p^{-1} \cdot q && \text{for } q : x_1 = a, \\ \text{transport}^{x \mapsto (x=x)}(p, q) &= p^{-1} \cdot q \cdot p && \text{for } q : x_1 = x_1. \end{aligned}$$

**Theorem 2.11.3.** For  $f, g : A \rightarrow B$ , with  $p : a =_A a'$  and  $q : f(a) =_B g(a)$ , we have

$$\text{transport}^{x \mapsto f(x)=g(x)}(p, q) =_{f(a')=g(a')} (\text{ap}_f p)^{-1} \cdot q \cdot \text{ap}_g p.$$

**Theorem 2.11.4.** Let  $B : A \rightarrow \mathcal{U}$  and  $f, g : \prod_{(x:A)} B(x)$ , with  $p : a =_A a'$  and  $q : f(a) =_{B(a)} g(a)$ . Then we have

$$\text{transport}^{x \mapsto f(x)=g(x)}(p, q) = (\text{apd}_f(p))^{-1} \cdot \text{ap}_{(\text{transport}^B p)}(q) \cdot \text{apd}_g(p).$$

**Theorem 2.11.5.** For  $p : a =_A a'$  with  $q : a = a$  and  $r : a' = a'$ , we have

$$(\text{transport}^{x \mapsto (x=x)}(p, q) = r) \simeq (q \cdot p = p \cdot r).$$

## 2.12 Coproducts

**Theorem 2.12.1.** For all  $x : A + B$  we have  $(\text{inl}(a_0) = x) \simeq \text{code}(x)$ .

## 2.13 Natural numbers

We use the encode-decode method to characterize the path space of the natural numbers, which are also a positive type.

$$\text{code} : \mathbb{N} \rightarrow \mathbb{N} \rightarrow \mathcal{U},$$

defined by double recursion over  $\mathbb{N}$  as follows:

$$\begin{aligned} \text{code}(0, 0) &::= \mathbf{1} \\ \text{code}(\text{succ}(m), 0) &::= \mathbf{0} \\ \text{code}(0, \text{succ}(n)) &::= \mathbf{0} \\ \text{code}(\text{succ}(m), \text{succ}(n)) &::= \text{code}(m, n). \end{aligned}$$

We also define by recursion a dependent function  $r : \prod_{(n:\mathbb{N})} \text{code}(n, n)$ , with

$$\begin{aligned} r(0) &::= \star \\ r(\text{succ}(n)) &::= r(n). \end{aligned}$$

**Theorem 2.13.1.** For all  $m, n : \mathbb{N}$  we have  $(m = n) \simeq \text{code}(m, n)$ .

## 2.14 Example: equality of structures

**Definition 2.14.1.** Given a type  $A$ , the type  $\text{SemigroupStr}(A)$  of semigroup structures with carrier  $A$  is defined by

$$\text{SemigroupStr}(A) ::= \sum_{(m:A \rightarrow A \rightarrow A)} \prod_{(x,y,z:A)} m(x, m(y, z)) = m(m(x, y), z).$$

A **semigroup** is a type together with such a structure:

$$\text{Semigroup} ::= \sum_{A:\mathcal{U}} \text{SemigroupStr}(A)$$

### 2.14.1 Lifting equivalences

$$\text{transport}^{\text{SemigroupStr}}(\text{ua}(e)) : \text{SemigroupStr}(A) \rightarrow \text{SemigroupStr}(B).$$

Moreover, this map is an equivalence, because  $\text{transport}^C(\alpha)$  is always an equivalence with inverse  $\text{transport}^C(\alpha^{-1})$ , see Lemmas 2.1.3 and 2.3.7.

## 2.15 Universal properties

$$(X \rightarrow A \times B) \rightarrow (X \rightarrow A) \times (X \rightarrow B) \quad (2.15.1)$$

defined by  $f \mapsto (\text{pr}_1 \circ f, \text{pr}_2 \circ f)$ .

**Theorem 2.15.2.** (2.15.1) is an equivalence.

$$\left( \prod_{x:X} (A(x) \times B(x)) \right) \rightarrow \left( \prod_{x:X} A(x) \right) \times \left( \prod_{x:X} B(x) \right) \quad (2.15.3)$$

defined as before by  $f \mapsto (\text{pr}_1 \circ f, \text{pr}_2 \circ f)$ .

**Theorem 2.15.4.** (2.15.3) is an equivalence.

$$\left( \prod_{x:X} \sum_{(a:A(x))} P(x, a) \right) \rightarrow \left( \sum_{(g:\prod_{(x:X)} A(x))} \prod_{(x:X)} P(x, g(x)) \right). \quad (2.15.5)$$

**Theorem 2.15.6.** (2.15.5) is an equivalence.